#### 2.1.1

Show the following properties:

1. If there exists a function $g : B \to A$ such that $f \circ g = I_A$, then $f : A \to B$ is injective.

   > Assume $f$ is not injective. Then it must collapse two distinct elements into one, i.e. $\exists a_1, a_2 \in A$ such that $f(a_1) = f(a_2) = b$ and $a_1 \neq a_2$. But if $f \circ g = I_A$, then $g(f(a_1)) = g(b) = a_1$ _and_ $g(f(a_2)) = g(b) = a_2$. Since $a_1$ and $a_2$ are distinct, $g$ must be non-deterministic, so $g$ cannot be a function as claimed.
   
   If $f : A \to B$ is injective and $A \neq \emptyset$, then there exists a function $g : B \to A$ such that $f \circ g = I_A$.
   
   > Let $f^T = \{<b,a> | <a,b> \in f\}$. Since $f$ is injective, $f^T$ is a partial function (deterministic), and since $f$ is total and $f^T$ is a partial function, $f \circ f^T = I_A$.
   >
   > Let $g$ be any total function which extends $f^T$ (this can be done because $f^T$ is a partial function). Since $g$ extends $f^T$, $I_A \subset f \circ g$, and since $g$ is functional/deterministic (in particular on $range(f) = dom(f^T)$) and $I_A$ is total, $f \circ g = I_A$.

1. A function $f$ is surjective if and only if there exists a function $g : B \to A$ such that $g \circ f = I_B$.

   > Forward direction: for each $b \in B$, let $g(b) = a$ for _some_ $a \in f^{-1}(b)$. Since $f$ is surjective, $f^{-1}(b)$ is non-empty, so we can always pick some $a$, and so $g$ is a (total) function. And of course $f(g(b)) = b = I_B(b)$ for all $b \in B$.
   >
   > Backward direction: by contradiction, assume $f$ is not surjective. Then there exists $b \in B$ such that $f^{-1}(b) = \emptyset$. Nothing maps to $b$, so $f(g(b)) \neq b$, so $g \circ f \neq I_B$.

1. A function $f : A \to B$ is bijective if and only if there is a function $f^{-1}$ called its _inverse_ such that $f \circ f^{-1} = I_A$ and $f^{-1} \circ f = I_B$.
   > Forward direction: given $f$'s injectivity, we know from the problem on injectivity that any functional extension $g$ of $f^T$ satisfies $f \circ g = I_A$, and since $f$ is also surjective the only functional extension is trivially $f^T=f^{-1}$ itself. Furthermore, since $f$ is total and surjective, $f^{-1}$ is as well, and because $(f^T)^T = f$, by symmetry we have $f^{-1} \circ f = I_B$.
   >
   > Backward direction: we know from the problems on injectivity and surjectivity that both $f$ and $f^{-1}$ are both injective and surjective, and are therefore bijective.
   
#### 2.1.2